CertiGC/verif_make_tinfo.v
@@ -7,10 +7,9 @@ Proof.
   Intros vret. destruct vret as [h p]. simpl fst. simpl snd.
   forward_call (thread_info_type, gv).
   Intros t. if_tac.
-  - subst t. forward_if False.
-    2: exfalso; first [rewrite Int64.eq_true in H; inversion H | apply H; trivial].
+  - subst t. forward_if False; [ | congruence].
     unfold all_string_constants; Intros; forward_call; contradiction.
   - Intros. forward_if True; [contradiction | forward; entailer! |]. Intros.
     forward. forward. rewrite Znth_0_cons. forward. forward. rewrite Znth_0_cons.
-    forward. forward. Exists t h p. entailer!.
+    forward. forward. forward. forward. forward. Exists t h p. entailer!.
 Qed.
